HOL-Light: Avoid hardcoded lengths in HOL-Light proof scripts
Previously, the HOL-Light proof scripts contained various hardcoded
constants related to the length of the code under proof, as well as
the lengths of preamble and postamble (stack spill and restore).

This commit replaces those hardcoded numerals with symbolic definitions.
As a result, SLOTHY re-optimization should now no longer require a proof
script change beyond the update of the byte code which is done by `autogen`
already.

Signed-off-by: Hanno Becker <beckphan@amazon.co.uk>

proofs/hol_light/arm/proofs/mlkem_rej_uniform.ml
@@ -176,6 +176,32 @@ let mlkem_rej_uniform_mc = define_assert_from_elf
 let MLKEM_REJ_UNIFORM_EXEC = ARM_MK_EXEC_RULE mlkem_rej_uniform_mc;;
 
 (* ------------------------------------------------------------------------- *)
+(* Code length constants                                                     *)
+(* ------------------------------------------------------------------------- *)
+
+let LENGTH_MLKEM_REJ_UNIFORM_MC =
+  REWRITE_CONV[mlkem_rej_uniform_mc] `LENGTH mlkem_rej_uniform_mc`
+  |> CONV_RULE (RAND_CONV LENGTH_CONV);;
+
+let MLKEM_REJ_UNIFORM_PREAMBLE_LENGTH = new_definition
+  `MLKEM_REJ_UNIFORM_PREAMBLE_LENGTH = 4`;;
+
+let MLKEM_REJ_UNIFORM_POSTAMBLE_LENGTH = new_definition
+  `MLKEM_REJ_UNIFORM_POSTAMBLE_LENGTH = 8`;;
+
+let MLKEM_REJ_UNIFORM_CORE_START = new_definition
+  `MLKEM_REJ_UNIFORM_CORE_START = MLKEM_REJ_UNIFORM_PREAMBLE_LENGTH`;;
+
+let MLKEM_REJ_UNIFORM_CORE_END = new_definition
+  `MLKEM_REJ_UNIFORM_CORE_END = LENGTH mlkem_rej_uniform_mc - MLKEM_REJ_UNIFORM_POSTAMBLE_LENGTH`;;
+
+let LENGTH_SIMPLIFY_CONV =
+  REWRITE_CONV[LENGTH_MLKEM_REJ_UNIFORM_MC;
+              MLKEM_REJ_UNIFORM_CORE_START; MLKEM_REJ_UNIFORM_CORE_END;
+              MLKEM_REJ_UNIFORM_PREAMBLE_LENGTH; MLKEM_REJ_UNIFORM_POSTAMBLE_LENGTH] THENC
+  NUM_REDUCE_CONV THENC REWRITE_CONV [ADD_0];;
+
+(* ------------------------------------------------------------------------- *)
 (* This is a general concept that subsumes a lot of specific cases like      *)
 (* num_of_bytelist and bignum_of_wordlist - should standardize a bit.        *)
 (* ------------------------------------------------------------------------- *)
@@ -462,19 +488,19 @@ let MLKEM_REJ_UNIFORM_CORRECT = prove
         24 divides val buflen /\
         8 * val buflen = 12 * LENGTH inlist /\
         ALL (nonoverlapping (stackpointer,576))
-            [(word pc,0x258); (buf,val buflen); (table,4096)] /\
+            [(word pc,LENGTH mlkem_rej_uniform_mc); (buf,val buflen); (table,4096)] /\
         ALL (nonoverlapping (res,512))
-            [(word pc,0x258); (stackpointer,576)]
+            [(word pc,LENGTH mlkem_rej_uniform_mc); (stackpointer,576)]
         ==> ensures arm
              (\s. aligned_bytes_loaded s (word pc) mlkem_rej_uniform_mc /\
-                  read PC s = word(pc + 0x4) /\
+                  read PC s = word(pc + MLKEM_REJ_UNIFORM_CORE_START) /\
                   read SP s = stackpointer /\
                   C_ARGUMENTS [res;buf;buflen;table] s /\
                   read(memory :> bytes(table,4096)) s =
                   num_of_wordlist mlkem_rej_uniform_table /\
                   read(memory :> bytes(buf,val buflen)) s =
                   num_of_wordlist inlist)
-             (\s. read PC s = word(pc + 0x250) /\
+             (\s. read PC s = word(pc + MLKEM_REJ_UNIFORM_CORE_END) /\
                   let outlist = SUB_LIST(0,256) (REJ_SAMPLE inlist) in
                   let outlen = LENGTH outlist in
                   C_RETURN s = word outlen /\
@@ -483,6 +509,7 @@ let MLKEM_REJ_UNIFORM_CORRECT = prove
              (MAYCHANGE_REGS_AND_FLAGS_PERMITTED_BY_ABI ,,
               MAYCHANGE [memory :> bytes(res,512);
                          memory :> bytes(stackpointer,576)])`,
+  CONV_TAC LENGTH_SIMPLIFY_CONV THEN
   MAP_EVERY X_GEN_TAC [`res:int64`; `buf:int64`] THEN
   W64_GEN_TAC `buflen:num` THEN
   MAP_EVERY X_GEN_TAC
@@ -1611,9 +1638,9 @@ let MLKEM_REJ_UNIFORM_SUBROUTINE_CORRECT = prove
         24 divides val buflen /\
         8 * val buflen = 12 * LENGTH inlist /\
         ALL (nonoverlapping (word_sub stackpointer (word 576),576))
-            [(word pc,0x258); (buf,val buflen); (table,4096)] /\
+            [(word pc,LENGTH mlkem_rej_uniform_mc); (buf,val buflen); (table,4096)] /\
         ALL (nonoverlapping (res,512))
-            [(word pc,0x258); (word_sub stackpointer (word 576),576)]
+            [(word pc,LENGTH mlkem_rej_uniform_mc); (word_sub stackpointer (word 576),576)]
         ==> ensures arm
              (\s. aligned_bytes_loaded s (word pc) mlkem_rej_uniform_mc /\
                   read PC s = word pc /\
@@ -1633,7 +1660,8 @@ let MLKEM_REJ_UNIFORM_SUBROUTINE_CORRECT = prove
              (MAYCHANGE_REGS_AND_FLAGS_PERMITTED_BY_ABI ,,
               MAYCHANGE [memory :> bytes(res,512);
                          memory :> bytes(word_sub stackpointer (word 576),576)])`,
+  CONV_TAC LENGTH_SIMPLIFY_CONV THEN
   CONV_TAC(TOP_DEPTH_CONV let_CONV) THEN
   ARM_ADD_RETURN_STACK_TAC MLKEM_REJ_UNIFORM_EXEC
-   (CONV_RULE (TOP_DEPTH_CONV let_CONV) MLKEM_REJ_UNIFORM_CORRECT)
+   (CONV_RULE (TOP_DEPTH_CONV let_CONV) (CONV_RULE LENGTH_SIMPLIFY_CONV MLKEM_REJ_UNIFORM_CORRECT))
     `[]:int64 list` 576);;
