proofs/hol_light/arm/proofs/mlkem_poly_basemul_acc_montgomery_cached_k4.ml
@@ -336,6 +336,16 @@ let basemul4_odd = define
 
   let poly_basemul_acc_montgomery_cached_k4_EXEC = ARM_MK_EXEC_RULE poly_basemul_acc_montgomery_cached_k4_mc;;
 
+ (* ------------------------------------------------------------------------- *)
+ (* Code length constants                                                     *)
+ (* ------------------------------------------------------------------------- *)
+
+ let LENGTH_POLY_BASEMUL_ACC_MONTGOMERY_CACHED_K4_MC =
+   REWRITE_CONV[poly_basemul_acc_montgomery_cached_k4_mc] `LENGTH poly_basemul_acc_montgomery_cached_k4_mc`
+   |> CONV_RULE (RAND_CONV LENGTH_CONV);;
+
+ let LENGTH_SIMPLIFY_CONV =
+   REWRITE_CONV[LENGTH_POLY_BASEMUL_ACC_MONTGOMERY_CACHED_K4_MC];;
 
  (* ------------------------------------------------------------------------- *)
  (* Hacky tweaking conversion to write away non-free state component reads.   *)
@@ -444,6 +454,7 @@ let basemul4_odd = define
    (* ------------------------------------------------------------------------- *)
 
   let poly_basemul_acc_montgomery_cached_k4_SPEC = prove(poly_basemul_acc_montgomery_cached_k4_GOAL,
+        CONV_TAC LENGTH_SIMPLIFY_CONV THEN
         REWRITE_TAC [MAYCHANGE_REGS_AND_FLAGS_PERMITTED_BY_ABI;
          MODIFIABLE_SIMD_REGS;
          NONOVERLAPPING_CLAUSES; ALL; C_ARGUMENTS; fst poly_basemul_acc_montgomery_cached_k4_EXEC] THEN
